CAinjp refinement proofed

demo/CA.v
@@ -4,45 +4,18 @@ Require Import Values Memory.
 Require Import Conventions Mach Asm.
 Require Import CKLR.
 Require Import Locations CallConv Compiler.
-
+Require Import InjectFootprint.
 
 (*
-Given b.asm
-
-
- sth
-
- CA -->> CA
-
- {| b.asm |}
-
-CCO:
-m             A                    m
-
-m_            cc_stacking injp   inj
-
-args_remove
-tm           B                   tm
-
- C  -> []
-
      injp
-
  C  -> [sp bx ra] li_c -> li_c   (cq : args m)
-
      CA
-
  Asm -> [sp bx ra]
-
-
-
    cc_c_asm_injp   ==    injp      === injp
                           CA           CL
                                        LM
                                        MA
-
 *)
-
 Record cc_ca_world :=
   caw{
       caw_sg : signature;
@@ -85,9 +58,6 @@ Inductive cc_c_asm_mr : cc_ca_world -> c_reply -> reply li_asm -> Prop :=
   cc_c_asm_mr_intro sg res tm m' tm' (rs rs' :regset) :
      let sp := rs#SP in
      res = rs_getpair (map_rpair preg_of (loc_result sg)) rs' ->
-(*     res = Locmap.getpair (map_rpair R (loc_result sg)) ls' ->
-     (forall r, In r (regs_of_rpair (loc_result sg)) -> rs' (preg_of r) = ls' (R r)) ->
-*)
      (forall r, is_callee_save r = true -> rs' (preg_of r) = rs (preg_of r)) ->
      Mem.unchanged_on (not_init_args (size_arguments sg) sp) m' tm' ->
      Mem.unchanged_on (loc_init_args (size_arguments sg) sp) tm tm' ->
@@ -148,7 +118,7 @@ Proof.
     apply Axioms.extensionality.
     intro r. destruct r; simpl; eauto.
   - intros r1 r2 Hr. inv Hr.
-    set (ls' loc := 
+    set (ls' loc :=
            match loc with
              |R r => rs' (preg_of r)
              |_ => Vundef
@@ -163,3 +133,383 @@ Proof.
     constructor; eauto.
     inversion H8. eauto.
 Qed.
+
+
+(** cc_c_asm_injp as a whole calling convention *)
+
+Record cc_cainjp_world :=
+  cajw {
+      cajw_injp: world injp;
+      cajw_sg : signature;
+      cajw_rs : regset;
+      cajw_m : mem
+    }.
+
+Inductive cc_c_asm_injp_mq : cc_cainjp_world -> c_query -> query li_asm -> Prop:=
+  cc_c_asm_injp_mq_intro sg args m j (rs: regset) tm tm0 vf
+    (Hm: Mem.inject j m tm):
+    let tsp := rs#SP in let tra := rs#RA in let tvf := rs#PC in
+    let targs := (map (fun p => Locmap.getpair p (make_locset_rs rs tm tsp))
+                      (loc_arguments sg)) in
+    Val.inject_list j args targs ->
+    Val.inject j vf tvf ->
+    (forall b ofs, loc_init_args (size_arguments sg) tsp b ofs ->
+              loc_out_of_reach j m b ofs) ->
+    Val.has_type tsp Tptr ->
+    Val.has_type tra Tptr ->
+    valid_blockv (Mem.support tm) tsp ->
+    args_removed sg tsp tm tm0 -> (* The Outgoing arguments are readable and freeable in tm *)
+    vf <> Vundef -> tra <> Vundef ->
+    cc_c_asm_injp_mq
+      (cajw (injpw j m tm Hm) sg rs tm)
+      (cq vf sg args m)
+      (rs,tm).
+
+Inductive cc_c_asm_injp_mr : cc_cainjp_world -> c_reply -> reply li_asm -> Prop :=
+  cc_c_asm_injp_mr_intro sg res j m tm Hm j' m' tm' Hm' (rs rs' :regset) :
+     let tsp := rs#SP in
+     let tres := rs_getpair (map_rpair preg_of (loc_result sg)) rs' in
+     Val.inject j' res tres ->
+     injp_acc (injpw j m tm Hm) (injpw j' m' tm' Hm') ->
+     (forall r, is_callee_save r = true -> rs' (preg_of r) = rs (preg_of r)) ->
+     (forall b ofs, loc_init_args (size_arguments sg) tsp b ofs ->
+              loc_out_of_reach j m b ofs) ->
+     rs'#SP = rs#SP -> rs'#PC = rs#RA ->
+     cc_c_asm_injp_mr
+       (cajw (injpw j m tm Hm) sg rs tm)
+       (cr res m')
+       (rs', tm').
+
+Program Definition cc_c_asm_injp : callconv li_c li_asm :=
+  {|
+    match_senv w := match_stbls injp (cajw_injp w);
+    match_query := cc_c_asm_injp_mq;
+    match_reply := cc_c_asm_injp_mr
+  |}.
+Next Obligation.
+  inv H. inv H1. eauto.
+Qed.
+Next Obligation.
+  inv H.
+  eapply Genv.valid_for_match in H2.
+  apply H2. eauto.
+Qed.
+
+Lemma cc_injpca_cainjp :
+  ccref (cc_c injp @ cc_c_asm) (cc_c_asm_injp).
+Proof.
+  intros [[se2 [j m tm Hm']] [sg rs]] se1 se2' q1 q2 Hse Hq.
+  destruct Hse. inv H. destruct H0.
+  destruct Hq as [q1' [Hq1 Hq2]]. cbn in *.
+  inv Hq1. cbn in *. inv H1. rename m1 into m. rename m2 into tm0.
+  inv Hq2. cbn in *. rename caw_m0 into tm. rename sg0 into sg.
+  inv H14.
+  - (*easy: no Outgoing part*)
+    rename tm0 into tm.
+    exists (cajw (injpw j m tm Hm3) sg rs tm).
+    repeat apply conj; eauto.
+    + constructor; eauto.
+    + econstructor; eauto.
+      intros. inv H3. red in H1. rewrite H1 in H6. extlia.
+      constructor; eauto.
+    + intros r1 r2 Hr. inversion Hr. subst. clear H11.
+      exists (cr tres tm'). split.
+      * econstructor; eauto. split.
+        instantiate (1:= injpw j' m' tm' Hm'0).
+        inv H15.
+        constructor; eauto.
+        constructor; eauto.
+        constructor; eauto.
+      * constructor; eauto with mem.
+        inv H15.
+        eapply Mem.unchanged_on_implies; eauto.
+        intros. inv H3. red in H1. rewrite H1 in H6. extlia.
+  - (*with Outgoing part*)
+    assert (Htm: Mem.inject j m tm).
+    { clear - Hm3 H3. inversion Hm3.
+      constructor; eauto.
+      - inversion  mi_inj.
+        constructor; eauto.
+        + intros. eapply Mem.perm_free_3; eauto.
+        + intros. assert (Mem.mem_contents tm0 = Mem.mem_contents tm).
+          apply Mem.free_result in H3. rewrite H3. cbn. reflexivity.
+          rewrite <- H1. eauto.
+      - intros. unfold Mem.valid_block in *.
+        erewrite <- Mem.support_free; eauto.
+      - intros.
+        eapply Mem.perm_free_inv in H0 as PERM; eauto.
+        destruct PERM.
+        + (* in freed region -> Source no perm *)
+          right. intro. destruct H1 as [Hb Hofs]. subst b2.
+          exploit Mem.perm_inject; eauto. intro PERMtm0.
+          eapply Mem.perm_free_2 in H3 as NOPERMtm0; eauto.
+        + eapply mi_perm_inv; eauto.
+    }
+    exists (cajw (injpw j m tm Htm) sg rs tm).
+    repeat apply conj; eauto.
+    + constructor; eauto.
+      erewrite <- Mem.support_free; eauto.
+    + econstructor; eauto.
+      * intros. inv H10. subst sp. rewrite <- H1 in H11. inv H11.
+        eapply Mem.perm_free_2 in H3 as NOPERM; eauto.
+        red. intros. intro.
+        exploit Mem.perm_inject. apply H10. apply Hm3.  eauto.
+        intros. replace (ofs - delta + delta) with ofs in H13 by lia.
+        apply NOPERM. eauto with mem.
+      * subst sp. rewrite <- H1.
+        eapply args_removed_free; eauto.
+    + intros r1 r2 Hr. inv Hr. clear H15. subst sp tsp. inv H24.
+      assert {tm'0| Mem.free tm' sb (offset_sarg sofs 0) (offset_sarg sofs (size_arguments sg)) = Some tm'0}.
+      {
+        apply Mem.range_perm_free.
+        red. intros.
+        apply Mem.free_range_perm in H3 as RANGEtm. red in RANGEtm.
+        inversion H30.
+        eapply unchanged_on_perm; eauto. apply H26. rewrite <- H1.
+        constructor; eauto. rewrite <- H1 in H18. inv H18. eauto.
+      }
+      destruct X as [tm'0 FREE'].
+      assert (INJ' : Mem.inject j' m' tm'0).
+      {
+        eapply Mem.free_right_inject; eauto. intros.
+        assert (loc_out_of_reach j' m' sb (ofs+ delta)).
+        eapply loc_out_of_reach_incr; eauto.
+        eapply H26; eauto. rewrite <- H1. econstructor; eauto.
+        eapply inject_implies_dom_in; eauto.
+        inv H18. rewrite <- H1 in H13. inv H13. eauto.
+        red in H13. exploit H13; eauto. replace (ofs + delta - delta) with ofs by lia.
+        eauto with mem.
+      }
+      exists (cr tres tm'0). repeat apply conj; eauto.
+      * econstructor. split.
+        instantiate (1:= injpw j' m' tm'0 INJ').
+        -- constructor; eauto.
+           ++ red. intros. red in H23.
+              exploit Mem.perm_free_3; eauto. intro PERMtm'.
+              exploit H23; eauto. unfold Mem.valid_block.
+              erewrite <- Mem.support_free; eauto.
+              intro PERMtm.
+              eapply Mem.perm_free_1; eauto.
+              eapply Mem.perm_free_4; eauto.
+           ++ exploit Mem.free_mapped_unchanged_on; eauto. (*change this*)
+              intros. eapply H26; eauto. rewrite <- H1. constructor; eauto.
+              intros [tm''0 [FREE'' UNC]].
+              rewrite FREE' in FREE''. inv FREE''. eauto.
+          ++ red. intros. exploit H32; eauto. intros [A B].
+             split; eauto with mem.
+        -- constructor; eauto. constructor.
+      * constructor; eauto.
+        -- eapply Mem.free_unchanged_on'; eauto.
+           intros. intro. red in H11. apply H11.
+           rewrite <- H1. constructor; eauto.
+        -- eapply Mem.unchanged_on_implies; eauto.
+        -- erewrite Mem.support_free. reflexivity. eauto.
+        -- intros. rewrite <- H1 in H10. inv H10.
+           eapply Mem.perm_free_2; eauto.
+Qed.
+
+Theorem loc_init_args_dec:
+  forall sz sp b ofs,
+    {loc_init_args sz sp b ofs} + {not_init_args sz sp b ofs}.
+Proof.
+  intros. destruct sp.
+  right; intro; inv H. 
+  right; intro; inv H.
+  right; intro; inv H.
+  right; intro; inv H.
+  right; intro; inv H.
+  destruct (eq_block b0 b). subst.
+  destruct (zle (offset_sarg i 0) ofs);
+  destruct (zlt ofs (offset_sarg i sz)).
+  left. constructor; eauto.
+  right. intro. inv H. extlia.
+  right. intro. inv H. extlia.
+  right. intro. inv H. extlia.
+  right. intro. inv H. congruence.
+Qed.
+
+(*directly used in later proof*)
+Lemma not_init_args_dec:
+  forall sz sp b ofs,
+    {not_init_args sz sp b ofs} + {~not_init_args sz sp b ofs}.
+Proof.
+  intros. destruct (loc_init_args_dec sz sp b ofs).
+  right. red. auto. left. auto.
+Qed.
+
+Lemma not_init_args_expand:
+  forall sz b ofs sb sofs,
+    not_init_args sz (Vptr sb sofs) b ofs ->
+    b <> sb \/ ofs < offset_sarg sofs 0
+    \/ offset_sarg sofs sz <= ofs.
+Proof.
+  intros.
+  red in H.
+  destruct (eq_block b sb); destruct (zlt ofs (offset_sarg sofs 0));
+    destruct (zle (offset_sarg sofs sz ) ofs ); intuition eauto.
+  exfalso. eapply H. subst. constructor; eauto. lia.
+Qed.
+
+Lemma no_perm_out_of_reach:
+  forall j m1 m2 b ofs,
+    Mem.inject j m1 m2 ->
+    (forall k p, ~ Mem.perm m2 b ofs k p) ->
+    loc_out_of_reach j m1 b ofs.
+Proof.
+  intros. red. intros.
+  intro. eapply Mem.perm_inject in H2; eauto.
+  replace (ofs - delta + delta) with ofs in H2 by lia.
+  eapply H0; eauto.
+Qed.
+
+Lemma inject_unchanged_on_inject:
+  forall j m1 m2 m3 P,
+    Mem.inject j m1 m2 ->
+    Mem.unchanged_on P m2 m3 ->
+    (forall b ofs, {P b ofs} + {~ P b ofs}) ->
+    (forall b ofs, ~ P b ofs -> loc_out_of_reach j m1 b ofs) ->
+    Mem.inject j m1 m3.
+Proof.
+  intros. inversion H. inversion H0.
+  intros. constructor; eauto.
+  - inversion mi_inj. constructor; eauto.
+    + intros. eapply unchanged_on_perm; eauto.
+      edestruct H1; eauto. apply H2 in n. red in n. exfalso.
+      eapply n; eauto. replace (ofs + delta - delta) with ofs by lia. eauto with mem.
+    + intros. erewrite unchanged_on_contents; eauto.
+      edestruct H1; eauto. apply H2 in n. red in n. exfalso.
+      eapply n; eauto. replace (ofs + delta - delta) with ofs by lia. eauto with mem.
+  - intros. unfold Mem.valid_block in *. eauto with mem.
+  - intros. destruct (Mem.perm_dec m1 b1 ofs Max Nonempty); eauto.
+    left. eapply unchanged_on_perm in H4; eauto.
+    exploit mi_perm_inv; eauto.
+    intros [A|B]. auto. congruence.
+    edestruct H1; eauto. apply H2 in n. red in n. exfalso.
+    eapply n; eauto. replace (ofs + delta - delta) with ofs by lia.
+    auto.
+Qed.
+
+Lemma cc_cainjp__injp_ca :
+  ccref (cc_c_asm_injp) (cc_c injp @ cc_c_asm).
+Proof.
+  intros [w sg rs tm] se1 se2 q1 q2 Hse Hq.
+  destruct w as [j m tm1 Hm]. inv Hse. inv Hq.
+  rename tm2 into tm0. inv H16.
+  - (* no Outgoing part*) rename tm0 into tm.
+    exists (se2, (injpw j m tm Hm), caw sg rs tm). repeat apply conj; eauto.
+    + constructor; eauto. constructor; eauto. constructor; eauto.
+    + econstructor; eauto. split.
+      econstructor; eauto. constructor.
+      econstructor; eauto. subst tsp0. eauto. constructor; eauto.
+      subst tvf. inv H9; try congruence.
+    + intros r1 r3 [r2 [Hr1 Hr2]]. destruct Hr1 as [w' [Hw Hr1]]. inv Hr1. inv Hr2.
+      cbn in *. destruct w' as [j' m' tm'' Hm']. inv Hw. cbn in *.
+      rename m2' into tm'0. inv H1. rename m1' into m'.
+      assert (Htm': Mem.inject j' m' tm').
+      {
+        clear - H20 Hm11 H24.
+        eapply inject_unchanged_on_inject; eauto.
+        apply not_init_args_dec.
+        intros. eapply no_perm_out_of_reach; eauto.
+        intros. red in H. eapply H24.
+        edestruct loc_init_args_dec; eauto. exfalso. eauto.
+      }
+      econstructor; eauto. instantiate (1:= Htm').
+      * constructor; eauto.
+        -- red. intros. destruct (loc_init_args_dec (size_arguments sg) sp b ofs).
+           ++ (* in the Outgoing arguments region *)
+             inversion H21. eapply unchanged_on_perm; eauto.
+           ++ red in H27. eapply H27; eauto.
+              inversion H20. eapply unchanged_on_perm; eauto.
+              inversion H29. unfold Mem.valid_block in *. eauto with mem.
+        -- constructor.
+           ++ rewrite <- H22. inversion H29. eauto.
+           ++ intros.
+              destruct (loc_init_args_dec (size_arguments sg) sp b ofs).
+              ** inversion H21. eauto.
+              ** etransitivity. inversion H29. eauto.
+                 inversion H20. eapply unchanged_on_perm; eauto.
+                 inversion H29. unfold Mem.valid_block in *. eauto with mem.
+           ++ intros.
+              destruct (loc_init_args_dec (size_arguments sg) sp b ofs).
+              ** inversion H21. eauto.
+              ** etransitivity. inversion H20.
+                 eapply unchanged_on_contents; eauto.
+                 inversion H29.
+                 eapply unchanged_on_perm0; eauto with mem.
+                 inversion H29. eauto.
+  - (* with Outgoing part *)
+    assert (Htm0: Mem.inject j m tm0).
+    {
+      eapply Mem.free_right_inject; eauto. intros.
+      red in H10. exploit H10; eauto. subst tsp0. rewrite <- H.
+      econstructor; eauto.
+      replace (ofs + delta - delta) with ofs by lia.
+      eauto with mem.
+    }
+    exists (se2, (injpw j m tm0 Htm0), caw sg rs tm). repeat apply conj; eauto.
+    + constructor; eauto. constructor; eauto. erewrite Mem.support_free; eauto.
+      constructor; eauto.
+    + econstructor; eauto. split.
+      econstructor; eauto. constructor.
+      econstructor; eauto. constructor. subst tsp0.
+      rewrite <- H. econstructor; eauto. subst tvf. inv H9; try congruence.
+    + intros r1 r3 [r2 [Hr1 Hr2]]. destruct Hr1 as [w' [Hw Hr1]]. inv Hr1. inv Hr2.
+      destruct w' as [j' m' tm'' Hm']. inv Hw.
+      rename m2' into tm'0. inv H12. rename m1' into m'. cbn in H7.
+      assert (Htm': Mem.inject j' m' tm').
+      {
+        eapply inject_unchanged_on_inject; eauto.
+        apply not_init_args_dec.
+        intros. eapply no_perm_out_of_reach; eauto.
+        intros. eapply H28.
+        edestruct loc_init_args_dec; eauto. exfalso. eauto.
+      }
+      econstructor; eauto. instantiate (1:= Htm').
+      * constructor; eauto.
+        -- red. intros. destruct (loc_init_args_dec (size_arguments sg) sp b ofs).
+           ++ (* in the Outgoing arguments region *)
+             inversion H25. eapply unchanged_on_perm; eauto.
+           ++ eapply Mem.perm_free_3; eauto.
+              red in H31. eapply H31; eauto.
+              unfold Mem.valid_block in *. erewrite Mem.support_free; eauto.
+              inversion H24. eapply unchanged_on_perm; eauto.
+              unfold Mem.valid_block in *. rewrite H26.
+              eapply Mem.perm_valid_block; eauto.
+        -- constructor.
+           ++ rewrite <- H26. erewrite <- Mem.support_free. 2: eauto.
+              inversion H33. eauto.
+           ++ intros.
+              destruct (loc_init_args_dec (size_arguments sg) sp b ofs).
+              ** inversion H25. eauto.
+              ** etransitivity. instantiate (1:= Mem.perm tm0 b ofs k p).
+                 split; intro. eapply Mem.perm_free_1; eauto.
+                 subst sp tsp0. rewrite <- H in n.
+                 eapply not_init_args_expand; eauto.
+                 eapply Mem.perm_free_3; eauto.
+                 etransitivity. inversion H33. eapply unchanged_on_perm; eauto.
+                 unfold Mem.valid_block in *. erewrite Mem.support_free; eauto.
+                 inversion H24. eapply unchanged_on_perm; eauto.
+                 unfold Mem.valid_block in *. erewrite <- Mem.support_free in H13. 2: eauto.
+                 inversion H33; eauto.
+           ++ intros.
+              destruct (loc_init_args_dec (size_arguments sg) sp b ofs).
+              ** inversion H25. eauto.
+              ** etransitivity. inversion H24. eapply unchanged_on_contents; eauto.
+                 inversion H33. eapply unchanged_on_perm0; eauto.
+                 apply Mem.perm_valid_block in H13.
+                 eapply Mem.valid_block_free_1; eauto.
+                 eapply Mem.perm_free_1; eauto.
+                 subst sp tsp0. rewrite <- H in n.
+                 eapply not_init_args_expand; eauto.
+                 etransitivity. inversion H33. eapply unchanged_on_contents; eauto.
+                 eapply Mem.perm_free_1; eauto.
+                 subst sp tsp0. rewrite <- H in n.
+                 eapply not_init_args_expand; eauto.
+                 apply Mem.free_result in H0. rewrite H0. reflexivity.
+        -- red. intros. exploit H35; eauto. intros [A B].
+           split; eauto with mem.
+Qed.
+
+
+
